\documentclass{article}
\usepackage{amsmath, amsthm, amsfonts}
\usepackage{centernot}
\author{Mostafa Hassanein}
\title{
  MTH-684 Logic \\
  Assignment (4): Reasoning in Propositional Logic}
\date{23 October 2024}
\begin{document}

\maketitle
\newpage

\section*{4-2}
Prove that:
\begin{align*}
  \{ (A \implies B), \: ((B \lor C) \implies D), \: (E \land \lnot D) \}  \vdash (A \implies E)
\end{align*}

\begin{proof}

  \begin{align*}
    &1. (A \implies B) &&\text{(Hypothesis)} &&\\
    &2. ((B \lor C) \implies D) &&\text{(Hypothesis)} &&\\
    &3. (E \land \lnot D) &&\text{(Hypothesis)} &&\\
    &4. \lnot D &&\text{(3, SIM)} &&\\
    &5. \lnot (B \lor C) &&\text{(2, 4, MT)} &&\\
    &6. (\lnot A \lor B) &&\text{(1, IMP1)} &&\\
    &7. ((\lnot A \lor B) \lor C) &&\text{(6, AD)} &&\\
    &8. (\lnot A \lor (B \lor C)) &&\text{(7, GR)} &&\\
    &9. (A \implies (B \lor C)) &&\text{(8, IMP2)} &&\\
    &10. \lnot A &&\text{(5, 9, MT)} &&\\
    &11. (\lnot A \lor E) &&\text{(10, AD)} &&\\
    &12. (A \implies E) &&\text{(11, IMP2)} &&\\
  \end{align*}

\end{proof}

\end{document}