\documentclass{article}
\usepackage{amsmath, amsthm, amsfonts}
\usepackage{centernot}
\usepackage{derivative}
\author{Mostafa Hassanein}
\title{
  MTH-632 PDEs \\
  Assignment (6): \\ Chapter 10: Green's Functions}
\date{3 Jan 2025}
\begin{document}

\maketitle
\newpage

\section*{10.2.1}
\begin{align*}
  &u_{t} = u_{xx} + Q(x, t) 0, \quad 0\leq x \leq 1, \quad t > 0 &&\\
  &u(x, 0) = f(x) &&\\
  &u(0, t) = A(t) &&\\
  &u(1, t) = B(t).
\end{align*}
Obtain a solution of the form:
\begin{align*}
  u(x,t) = \int_{0}^{1} f(s) G(x;s,t) ds +
  \int_{0}^{1} \int_{0}^{t} Q(s,\tau) G(x; s, t-\tau) d\tau ds.  
\end{align*}

\begin{center}
  \noindent\rule{8cm}{0.4pt}
\end{center}

\underline{Solution:}
\begin{align*}
  &w(x, t) = A(t) + x[B(t) - A(t)] &&\\
  &v(x, t) = u(x, t) - w(x, t) &&\\
  &y(x, t) = Q(x, t) - wt + w_{xx}.
\end{align*}
\begin{align*}
  \implies&v_{t} = v_{xx} + y(x, t) &&\\
  &v(x, 0) = g(x) = f(x) - A(0) - x[B(0) - A(0)] &&\\
  &v(0, t) = v(1, t) = 0.
\end{align*}
\newline

The eigenfunctions are given by:
\begin{align*}
  &\phi_{n}(x) = sin(n \pi x) &&\\ 
  &\lambda_n = (n\pi)^2 &&\\ 
  &n= 1, 2, \ldots
\end{align*}

Expand $y(x,t)$ in the eigenfunction basis:
\begin{align*}
  &y(x,t) = \sum_{n=1}^{\infty} y_n(t) \phi_n(x) &&\\
  \implies&y_n(t) = \frac{\int_{0}^{1} y(x,y) \sin(n \pi x) dx}{\int_{0}^{1} \sin^2(n \pi x) dx}.
\end{align*}

Expand $v(x,t)$ in the eigenfunction basis:
\begin{align*}
  &v(x,t) = \sum_{n=1}^{\infty} v_n(t) \phi(x) &&\\
  \implies& v(x, 0) = \sum_{n=1}^{\infty} v_n(0) \phi_n(x) = g(x) &&\\
  \implies& v_n(0) = \frac{\int_{0}^{1} g(x) \sin(n \pi x) dx}{\int_{0}^{1} \sin^2(n \pi x) dx} 
  = 2 \int_{0}^{1} g(x) \sin(n \pi x) dx.
\end{align*}

Plugging into the PDE, we get:
\begin{align*}
  &\sum_{n=1}^{\infty} 
  \left[
    \dot{v}_n(t) + n^2 \pi^2 v_n(t) - y_n(t)
  \right] 
  \sin(n \pi x) = 0 &&\\
  \implies& \forall n: \dot{v}_n(t) + n^2 \pi^2 v_n(t) = y_n(t).
\end{align*}

Using the method of variation of parameters, we can solve for $v_n(t)$ as follows:
\begin{align*}
  v_n(t) 
  &= v_n(0) e^{- n^2 \pi ^2 t}
  + \int_{0}^{t} y_n(\tau) e^{-n^2 \pi^2 (t - \tau)} d\tau &&\\
  &= e^{- n^2 \pi ^2 t} 2 \int_{0}^{1} g(x) \sin(n \pi x) dx 
  + \int_{0}^{t} y_n(\tau) e^{-n^2 \pi^2 (t - \tau)} d\tau.
\end{align*}

Now, plugging into $v(x,t)$, we get:
\begin{align*}
  v(x,t) 
  &= \sum_{n=1}^{\infty} v_n(t) \phi(x) &&\\
  &=
  \sum_{n=1}^{\infty}
  \left[
    e^{- n^2 \pi ^2 t} 2 \int_{0}^{1} g(x) \sin(n \pi x) dx 
  + \int_{0}^{t} y_n(\tau) e^{-n^2 \pi^2 (t - \tau)} d\tau
  \right]
  \sin(n \pi x)
\end{align*}

\end{document}

